timesyn/CaseStudies/abp/Sender.thy
@@ -8,52 +8,9 @@
 chapter {* Theory for Sender Automaton Lemmata *}
 
 theory Sender
-imports SenderAutomaton 
+imports Components 
 
 begin
-
-(* ----------------------------------------------------------------------- *)
-  section {* Datatype Conversion *}
-(* ----------------------------------------------------------------------- *)
-
-text {* Inverse of a Pair. *}
-fun invPair :: "abpMessage \<Rightarrow> (nat \<times> bool)" where
-  "invPair (Pair_nat_bool (n,b)) = (n,b)" |
-  "invPair n = undefined"
-
-text {* Conversion of a pair (nat,bool) stream into an equivalent receiver stream. *}
-definition natbool2abp :: "(nat \<times> bool) tsyn stream \<rightarrow> abpMessage tsyn stream" where
-  "natbool2abp \<equiv> tsynMap Pair_nat_bool"
-
-text {* Conversion of a receiver stream into an equivalent pair (nat,bool) stream. *}
-definition abp2natbool :: "abpMessage tsyn stream \<rightarrow> (nat \<times> bool) tsyn stream" where
-  "abp2natbool \<equiv> tsynMap invPair"
-
-text {* Inverse of a Bool. *}
-fun invBool :: "abpMessage \<Rightarrow> bool" where
-  "invBool (Bool x) = x" |
-  "invBool x = undefined"
-
-text {* Conversion of a bool stream into an equivalent receiver stream. *}
-definition bool2abp :: "bool tsyn stream \<rightarrow> abpMessage tsyn stream" where
-  "bool2abp \<equiv> tsynMap Bool"
-
-text {* Conversion of a receiver stream into an equivalent bool stream. *}
-definition abp2bool :: "abpMessage tsyn stream \<rightarrow> bool tsyn stream" where
-  "abp2bool \<equiv> tsynMap invBool"
-
-text {* Inverse of a Nat. *}
-fun invNat :: "abpMessage \<Rightarrow> nat" where
-  "invNat (Nat x) = x" |
-  "invNat x = undefined"
-
-text {* Conversion of a nat stream into an equivalent receiver stream. *}
-definition nat2abp :: "nat tsyn stream \<rightarrow> abpMessage tsyn stream" where
-  "nat2abp \<equiv> tsynMap Nat"
-
-text {* Conversion of a receiver stream into an equivalent nat stream. *}
-definition abp2nat :: "abpMessage tsyn stream \<rightarrow> nat tsyn stream" where
-  "abp2nat \<equiv> tsynMap invNat"
 
 (* ----------------------------------------------------------------------- *)
   section {* Sender Test Streams and Bundles *}
